Adjusted trace arithmetic for changes from #92 to trace API

src/core/DY.Core.Trace.SplitUtils.Derived.fst
@@ -9,12 +9,12 @@ open DY.Core.Trace.SplitUtils
 
 /// Derived functions for trace split
 
-let trace_split_grows (#label_t:Type) (tr:trace_ label_t) (ts:timestamp {ts < length tr})
+let trace_split_grows (#label_t:Type) (tr:trace_ label_t) (ts:timestamp {ts `on_trace` tr})
   : Lemma
     (ensures (
       let (tr1, e, _) = trace_split tr ts in
       tr1 <$ tr /\
-      (Snoc tr1 e) <$ tr
+      (append_entry tr1 e) <$ tr
     ))
   = trace_split_matches_prefix tr ts
 
@@ -30,20 +30,20 @@ let trace_split_at (#a:Type) (tr:trace_ a) (e:trace_entry_ a{entry_exists tr e})
 
 let trace_subtract_nil (#label_t:Type) (tr:trace_ label_t)
   : Lemma
-    ((tr <--> Nil) == tr)
-    [SMTPat (tr <--> Nil)]
-  = trace_concat_subtract Nil tr
+    ((tr <--> empty_trace) == tr)
+    [SMTPat (tr <--> empty_trace)]
+  = trace_concat_subtract empty_trace tr
 
 let trace_subtract_itself (#label_t:Type) (tr:trace_ label_t)
   : Lemma
-    ((tr <--> tr) == Nil)
+    ((tr <--> tr) == empty_trace)
     [SMTPat (tr <--> tr)]
-  = trace_concat_subtract tr Nil
+  = trace_concat_subtract tr empty_trace
 
 let trace_concat_snoc_right (#label_t:Type) (tr1 tr2:trace_ label_t) (e:trace_entry_ label_t)
   : Lemma
-    (tr1 <++> (Snoc tr2 e) == Snoc (tr1 <++> tr2) e)
-  = trace_concat_assoc tr1 tr2 (Snoc Nil e)
+    (tr1 <++> (append_entry tr2 e) == append_entry (tr1 <++> tr2) e)
+  = trace_concat_assoc tr1 tr2 (append_entry empty_trace e)
 
 let trace_subtract_concat_left (#label_t:Type) (tr1 tr2 tr3:trace_ label_t)
   : Lemma
